tests/bug-reports/closed/Bug3865.fst
@@ -14,6 +14,8 @@ let intpak = {
   f = (fun x -> x + 1);
 }
 
+#push-options "--warn_error -272" //Warning_TopLevelEffect
 let use =
   let x = intpak.f 123 in
   IO.print_string (string_of_int x ^ "\n")
+#pop-options
